finish stlcprop main

TypeTheory/StlcProp.lean
@@ -1,9 +1,40 @@
+-- https://softwarefoundations.cis.upenn.edu/plf-current/StlcProp.html
+
 import TypeTheory.Stlc
 import Mathlib.Data.Finmap
 
 open STLC Finmap
 
 namespace STLC
+
+section destruct_has_type
+
+theorem var_type_in_context: ∀ {Γ x T},
+    (Γ ⊢ tm.tm_var x : T) → Γ.lookup x = some T :=
+  fun hx => by cases hx with | T_Var _ _ _ h => exact h
+
+theorem app_type_in_context: ∀ {Γ t1 t2 T2},
+    (Γ ⊢ tm.tm_app t1 t2 : T2) →
+      ∃ T1, (Γ ⊢ t1 : T1 → T2) ∧  (Γ ⊢ t2 : T1) :=
+  fun happ => by cases happ with | T_app _ _ _ _ _ h1 h2 => exact ⟨_, h1, h2⟩
+
+theorem if_type_in_context: ∀ {Γ t1 t2 t3 T},
+    (Γ ⊢ tm.tm_if t1 t2 t3 : T) →
+      (Γ ⊢ t1 : BOOL) ∧ (Γ ⊢ t2 : T) ∧ (Γ ⊢ t3 : T) :=
+  fun hif => by cases hif with | T_If _ _ _ _ _ h1 h2 h3 => exact ⟨h1, h2, h3⟩
+
+theorem abs_type_in_context: ∀ {Γ x Tx t T},
+    (Γ ⊢ tm.tm_abs x Tx t : T) →
+      (∃ Tt, T = (Tx → Tt) ∧ (Γ.insert x Tx ⊢ t : Tt)) :=
+  fun habs => by cases habs with | T_Abs _ _ _ Tt _ h => use Tt
+
+theorem true_type_in_context: ∀ {Γ T}, (Γ ⊢ tm.tm_true : T) → T = BOOL :=
+  fun h => by cases h with | T_True => rfl
+
+theorem false_type_in_context: ∀ {Γ T}, (Γ ⊢ tm.tm_false : T) → T = BOOL :=
+  fun h => by cases h with | T_False => rfl
+
+end destruct_has_type
 
 #check has_type.T_Var
 #check has_type.T_app
@@ -36,51 +67,44 @@ theorem progress:
   | tm_var s => intro T h; contradiction
   | tm_app s1 s2 ih1 ih2 =>
     intro T h
-    cases h with
-    | T_app _ s1 s2 T1 T2 h1 h2 =>
-      specialize ih1 (T1 → T) h1
-      specialize ih2 T1 h2
-      rcases ih1 with (hl | hr)
-      · let s1abs := canonical_forms_fun s1 T1 T h1 hl
-        rcases s1abs with ⟨x, u, rfl⟩
-        right
-        rcases ih2 with (h2l | ⟨s2', hs2'⟩)
-        · use u [x := s2]
-          apply step.ST_AppAbs
-          exact h2l
-        · use λ x: T1, u ↠ s2'
-          apply step.ST_App2
-          · exact value.v_abs x T1 u
-          assumption
-      · right
-        rcases hr with ⟨s1', hs1'⟩
-        use s1' ↠ s2
-        apply step.ST_App1
-        · exact hs1'
+    let ⟨T1, h1, h2⟩ := app_type_in_context h
+    specialize ih1 (T1 → T) h1
+    specialize ih2 T1 h2
+    rcases ih1 with (hl | hr)
+    · let s1abs := canonical_forms_fun s1 T1 T h1 hl
+      rcases s1abs with ⟨x, u, rfl⟩
+      right
+      rcases ih2 with (h2l | ⟨s2', hs2'⟩)
+      · exact ⟨u [x:=s2], step.ST_AppAbs x T1 u s2 h2l⟩
+      · use λ x: T1, u ↠ s2'
+        apply step.ST_App2
+        · exact value.v_abs x T1 u
+        exact hs2'
+    · right
+      rcases hr with ⟨s1', hs1'⟩
+      use s1' ↠ s2
+      apply step.ST_App1
+      exact hs1'
   | tm_abs x T t _ => exact fun T1 _ => Or.inl (value.v_abs x T t)
   | tm_true => exact fun T _ => Or.inl value.v_true
   | tm_false => exact fun T _ => Or.inl value.v_false
   | tm_if x t1 t2 ihx _ _ =>
     intro T h
     right
-    cases h with
-    | T_If _ x t1 t2 T hx ht1 ht2 =>
-      let hif := ihx BOOL hx
-      rcases hif with (hvaluex | ⟨x', hx'⟩)
-      · let xbool := canonical_forms_bool x hx hvaluex
-        rcases xbool with (xv | xv) <;> rw [xv]
-        · use t1
-          apply step.ST_IfTrue
-        · use t2
-          apply step.ST_IfFalse
-      · use <{If x' Then t1 Else t2}>
-        apply step.ST_If
-        exact hx'
+    let ⟨hx, _, _⟩ := if_type_in_context h
+    let hif := ihx BOOL hx
+    rcases hif with (hvaluex | ⟨x', hx'⟩)
+    · let xbool := canonical_forms_bool x hx hvaluex
+      rcases xbool with (rfl | rfl)
+      · exact ⟨t1, step.ST_IfTrue t1 t2⟩
+      · exact ⟨t2, step.ST_IfFalse t1 t2⟩
+    · use <{If x' Then t1 Else t2}>
+      exact step.ST_If x x' t1 t2 hx'
 
 open partialmap
 
 count_heartbeats in
-theorem weakening : ∀ Γ Γ' t T,
+theorem weakening : ∀ {Γ Γ' t T},
     includedin Γ Γ' → (Γ ⊢ t : T) → (Γ' ⊢ t : T) := by
   intro Γ Γ' t T h ht
   induction ht generalizing Γ' with
@@ -90,37 +114,97 @@ theorem weakening : ∀ Γ Γ' t T,
   | T_Abs Γ'' x T1 T2 t2 _ a_ih =>
     apply has_type.T_Abs
     let insertincluded := includedin_insert h x T1
-    exact (a_ih _ insertincluded)
+    exact (a_ih insertincluded)
   | T_app Γ'' t1 t2 T1 T2 _ _ a_iht1 a_iht2 =>
     refine has_type.T_app ?_ t1 t2 T1 T2 ?_1 ?_2
-    · exact a_iht1 _ h
-    · exact a_iht2 _ h
+    · exact a_iht1 h
+    · exact a_iht2 h
   | T_True => exact has_type.T_True _
   | T_False => exact has_type.T_False _
   | T_If Γ'' x t2 t3 T _ _ _ a_ihx a_iht2 a_iht3 =>
     refine has_type.T_If Γ' x t2 t3 T ?_ ?_ ?_3
-    · exact a_ihx _ h
-    · exact a_iht2 _ h
-    · exact a_iht3 _ h
+    · exact a_ihx h
+    · exact a_iht2 h
+    · exact a_iht3 h
 
-theorem weakening_empty : ∀ Γ t T,
+theorem weakening_empty : ∀ {Γ t T},
     (∅ ⊢ t : T) → (Γ ⊢ t : T) := by
   intro Γ t T ht
-  exact weakening _ _ _ _ (includedin_empty _) ht
+  exact weakening (includedin_empty _) ht
 
 theorem substitution_preserves_typing :
-  ∀ Γ x U t v T,
+  ∀ {Γ x U t v T},
     (Γ.insert x U ⊢ t : T) →
     (∅ ⊢ v : U) →
     (Γ ⊢ t [x := v] : T) := by
-  sorry
+  intro Γ x U t v T
+  intro ht
+  intro hv
+  induction t generalizing Γ T with
+  | tm_var y =>
+    dsimp [subst]
+    by_cases h: x=y
+    · subst_vars; rw [if_pos rfl]
+      apply var_type_in_context at ht
+      rw [lookup_insert] at ht
+      apply weakening_empty
+      injection ht; subst_vars; exact hv
+    · rw [if_neg h]
+      apply has_type.T_Var
+      apply var_type_in_context at ht
+      rw [lookup_insert_of_ne Γ (Ne.symm h)] at ht
+      exact ht
+  | tm_app t1 t2 ih1 ih2 =>
+    dsimp [subst]
+    let ⟨T1, ht1, ht2⟩ := app_type_in_context ht
+    apply has_type.T_app
+    · exact ih1 ht1
+    · exact ih2 ht2
+  | tm_abs y U' t' ih =>
+    dsimp [subst]
+    rcases abs_type_in_context ht with ⟨Tt', rfl, ht'⟩
+    by_cases h: x=y
+    · subst_vars; rw [if_pos rfl]
+      apply has_type.T_Abs
+      rw [insert_insert] at ht'
+      exact ht'
+    · rw [if_neg h]
+      apply has_type.T_Abs
+      apply ih
+      rw [insert_insert_of_ne _ (Ne.symm h)]
+      exact ht'
+  | tm_true =>
+    exact (true_type_in_context ht) ▸ has_type.T_True _
+  | tm_false =>
+    exact (false_type_in_context ht) ▸ has_type.T_False _
+  | tm_if y t1 t2 ih1 ih2 ih3 =>
+    dsimp [subst]
+    rcases if_type_in_context ht with ⟨ht1, ht2, ht3⟩
+    apply has_type.T_If _ _ _ _ _ (ih1 ht1) (ih2 ht2) (ih3 ht3)
 
 theorem preservation :
-  ∀ t t' T,
+  ∀ {t t' T},
     (∅ ⊢ t : T) →
     t ->- t' →
     (∅ ⊢ t' : T) := by
-  sorry
+  intro t t' T ht hr
+  induction hr generalizing T with
+  | ST_AppAbs x T2 t1 v2 _ =>
+    rcases app_type_in_context ht with ⟨T1, ht1, ht2⟩
+    rcases abs_type_in_context ht1 with ⟨Tt, hTt, ht1'⟩
+    injection hTt; subst_vars
+    exact substitution_preserves_typing ht1' ht2
+  | ST_App1 t1 t1' t2 _ a_ih =>
+    rcases app_type_in_context ht with ⟨T1, ht1, ht2⟩
+    exact has_type.T_app _ _ _ _ _ (a_ih ht1) ht2
+  | ST_App2 v1 t2 t2' _ _ a_ih =>
+    rcases app_type_in_context ht with ⟨T1, ht1, ht2⟩
+    exact has_type.T_app _ _ _ _ _ ht1 (a_ih ht2)
+  | ST_IfTrue t1 t2 => exact (if_type_in_context ht).2.1
+  | ST_IfFalse t1 t2 => exact (if_type_in_context ht).2.2
+  | ST_If t1 t1' t2 t3 _ a_ih =>
+    rcases if_type_in_context ht with ⟨ht1, ht2, ht3⟩
+    exact has_type.T_If _ _ _ _ _ (a_ih ht1) ht2 ht3
 
 theorem preservation' :
   ∀ t t' T,
@@ -130,16 +214,27 @@ theorem preservation' :
   intro t t' T ht htt'
   induction htt' generalizing T with
   | multi_refl t => exact ht
-  | multi_step x y z rxy syz a_ih =>
+  | multi_step x y _ rxy _ a_ih =>
     apply a_ih
-    exact preservation x y T ht rxy
-
-  sorry
+    exact preservation ht rxy
 
 theorem not_subject_expansion :
   ∃ t t' T,
     t ->- t' ∧ (∅ ⊢ t' : T) ∧ ¬ (∅ ⊢ t : T) := by
-  sorry
+  let t := <{λ x: (BOOL → BOOL), x ↠ TRUE}>
+  use t, <{TRUE}>, BOOL
+  constructor
+  · apply step.ST_AppAbs
+    apply value.v_true
+  constructor
+  · apply has_type.T_True
+  intro h
+  apply app_type_in_context at h
+  rcases h with ⟨T1, ht1, ht2⟩
+  apply abs_type_in_context at ht1
+  rcases ht1 with ⟨Tt, hTt, ht1'⟩
+  injection hTt; subst_vars
+  cases ht2
 
 def stuck (t : tm) : Prop :=
   (normal_form step) t ∧ ¬ value t
@@ -157,9 +252,38 @@ theorem type_soundness :
 theorem unique_types :
   ∀ Γ e T T',
     (Γ ⊢ e : T) → (Γ ⊢ e : T') → T = T' := by
-  sorry
+  intro Γ e T T'
+  intro hT hT'
+  induction e generalizing T T' Γ with
+  | tm_var x =>
+    apply var_type_in_context at hT
+    apply var_type_in_context at hT'
+    rw [hT] at hT'
+    exact Option.noConfusion hT' id
+  | tm_app t1 t2 a_ih1 _a_ih2 =>
+    rcases app_type_in_context hT with ⟨_, hT1, _⟩
+    rcases app_type_in_context hT' with ⟨_, hT1', _⟩
+    specialize a_ih1 _ _ _ hT1 hT1'
+    injection a_ih1
+  | tm_abs x T1 t2 a_ih =>
+    rcases abs_type_in_context hT with ⟨_, rfl, hT1⟩
+    rcases abs_type_in_context hT' with ⟨_, rfl, hT1'⟩
+    specialize a_ih _ _ _ hT1 hT1'
+    rw [a_ih]
+  | tm_true =>
+    apply true_type_in_context at hT
+    apply true_type_in_context at hT'
+    rw [hT, hT']
+  | tm_false =>
+    apply false_type_in_context at hT
+    apply false_type_in_context at hT'
+    rw [hT, hT']
+  | tm_if t1 t2 t3 _a_ih1 _a_ih2 a_ih3 =>
+    rcases if_type_in_context hT with ⟨_, _, hT3⟩
+    rcases if_type_in_context hT' with ⟨_, _, hT3'⟩
+    exact a_ih3 _ _ _ hT3 hT3'
 
-class inductive appears_free_in (x : String) : tm → Prop :=
+inductive appears_free_in (x : String) : tm → Prop :=
   | afi_var : appears_free_in x <{x}>
   | afi_app1 : ∀ t1 t2, appears_free_in x t1 → appears_free_in x <{t1 ↠ t2}>
   | afi_app2 : ∀ t1 t2, appears_free_in x t2 → appears_free_in x <{t1 ↠ t2}>
@@ -168,24 +292,100 @@ class inductive appears_free_in (x : String) : tm → Prop :=
   | afi_if2 : ∀ t1 t2 t3, appears_free_in x t2 → appears_free_in x <{If t1 Then t2 Else t3}>
   | afi_if3 : ∀ t1 t2 t3, appears_free_in x t3 → appears_free_in x <{If t1 Then t2 Else t3}>
 
-def closed (t : tm) : Prop :=
-  ∀ x, ¬ appears_free_in x t
+def closed (t : tm) : Prop := ∀ x, ¬ appears_free_in x t
 
 theorem free_in_context :
-  ∀ x t T Γ,
+  ∀ {x t T Γ},
     (appears_free_in x t) → (Γ ⊢ t : T) → (∃ U, Γ.lookup x = some U) := by
-  sorry
+  intro x t T Γ
+  intro h ht
+  induction h generalizing Γ T with
+  | afi_var => apply var_type_in_context at ht; use T
+  | afi_app1 t1 t2 _a a_ih =>
+    rcases app_type_in_context ht with ⟨T1, ht1, _ht2⟩
+    exact a_ih ht1
+  | afi_app2 t1 t2 _a a_ih =>
+    rcases app_type_in_context ht with ⟨T1, _ht1, ht2⟩
+    exact a_ih ht2
+  | afi_abs y Ty t h _h' a_ih =>
+    rcases abs_type_in_context ht with ⟨Tt, _hTt, ht'⟩
+    specialize a_ih ht'
+    exact (lookup_insert_of_ne _ h) ▸ a_ih
+  | afi_if1 t1 t2 t3 _a a_ih =>
+    rcases if_type_in_context ht with ⟨ht1, _ht2, _ht3⟩
+    exact a_ih ht1
+  | afi_if2 t1 t2 t3 _a a_ih =>
+    rcases if_type_in_context ht with ⟨_ht1, ht2, _ht3⟩
+    exact a_ih ht2
+  | afi_if3 t1 t2 t3 _a a_ih =>
+    rcases if_type_in_context ht with ⟨_ht1, _ht2, ht3⟩
+    exact a_ih ht3
 
 theorem typable_empty_closed :
   ∀ t T,
     (∅ ⊢ t : T) → closed t := by
-  sorry
+  intro t T ht
+  intro x h
+  let ⟨u, hu⟩ := free_in_context h ht
+  exact Option.noConfusion hu
+
+open appears_free_in
 
 theorem context_invariance :
-  ∀ Γ Γ' t T,
+  ∀ {Γ Γ' t T},
     (Γ ⊢ t : T) → (∀ x, appears_free_in x t → Γ.lookup x = Γ'.lookup x) → (Γ' ⊢ t : T) := by
-  sorry
+  intro Γ Γ' t T ht h
+  induction t generalizing Γ Γ' T with
+  | tm_var x =>
+    apply var_type_in_context at ht
+    apply has_type.T_Var
+    exact (h x (@afi_var x)) ▸ ht
+  | tm_app t1 t2 a_ih1 a_ih2 =>
+    rcases app_type_in_context ht with ⟨T1, ht1, ht2⟩
+    have sg1 : Γ' ⊢ t1 : T1 → T :=
+      a_ih1 ht1 fun x hafi => h x (afi_app1 t1 t2 hafi)
+    have sg2 : Γ' ⊢ t2 : T1 :=
+      a_ih2 ht2 fun x hafi => h x (afi_app2 t1 t2 hafi)
+    exact has_type.T_app _ _ _ _ _ sg1 sg2
+  | tm_abs x Tx t a_ih =>
+    rcases abs_type_in_context ht with ⟨Tt, rfl, ht'⟩
+    have sg1 : Finmap.insert x Tx Γ' ⊢ t : Tt := a_ih ht' fun y hafi => by
+      by_cases hxy : x = y
+      · subst_vars
+        repeat rw [lookup_insert]
+      · repeat rw [lookup_insert_of_ne _ (Ne.symm hxy)]
+        exact h y (afi_abs x Tx t (Ne.symm hxy) hafi)
+    exact has_type.T_Abs Γ' x Tx Tt t sg1
+  | tm_true => exact (true_type_in_context ht) ▸ has_type.T_True _
+  | tm_false => exact (false_type_in_context ht) ▸ has_type.T_False _
+  | tm_if t1 t2 t3 a_ih1 a_ih2 a_ih3 =>
+    rcases if_type_in_context ht with ⟨ht1, ht2, ht3⟩
+    have sg1 : Γ' ⊢ t1 : BOOL := a_ih1 ht1 fun x hafi => h x (afi_if1 t1 t2 t3 hafi)
+    have sg2 : Γ' ⊢ t2 : T := a_ih2 ht2 fun x hafi => h x (afi_if2 t1 t2 t3 hafi)
+    have sg3 : Γ' ⊢ t3 : T := a_ih3 ht3 fun x hafi => h x (afi_if3 t1 t2 t3 hafi)
+    exact has_type.T_If _ _ _ _ _ sg1 sg2 sg3
 
 end STLC
+
+namespace STLCArith
+
+inductive ty : Type :=
+  | Ty_Arrow : ty → ty → ty
+  | Ty_Nat : ty
+
+inductive tm : Type :=
+  | tm_var : String → tm
+  | tm_app : tm → tm → tm
+  | tm_abs : String → ty → tm → tm
+  | tm_const : Nat → tm
+  | tm_succ : tm → tm
+  | tm_pred : tm → tm
+  | tm_mult : tm → tm → tm
+  | tm_if₀ : tm → tm → tm → tm
+
+-- TODO !
+
+end STLCArith
+
 
 #check Finmap
