TypeTheory/Stlc.lean
@@ -1,3 +1,4 @@
+-- https://softwarefoundations.cis.upenn.edu/plf-current/Stlc.html
 import Mathlib.Data.Finmap
 
 set_option diagnostics.threshold 100
